Upd 2pm

temp/Spec.Claim.MerkleTree.fst
@@ -1,7 +1,8 @@
-module M
-open FStar.List.Tot
+module Spec.Claim.MerkleTree
+
 open FStar.Seq
-open FStar.UInt8
+open FStar.Mul
+open FStar.List.Tot
 
 type bytes = seq nat
 type hash_t = bytes
@@ -18,4 +19,78 @@ type merkleTree (#a : eqtype) : nat -> hash_t ->Type =
         merkleTree #a (level+1) (concat h1 h2)
 
 
-val merkleTreeGeneration       
+type merklePair (#a: eqtype) (n:nat) = h:hash_t & (merkleTree #a n h)
+
+
+val _merkleTreeGenerationL0: #a: eqtype -> l:list a -> Tot (r: list (merklePair #a 0){List.length l = List.length r})
+        (decreases (List.length l))
+
+let rec _merkleTreeGenerationL0 #a l = 
+    match l with
+    | hd1:: tl ->let h = hash hd1 in 
+                    let element = (|h, MLeaf hd1|)
+                    in  List.append [element] (_merkleTreeGenerationL0 #a tl)
+    | [] -> [] 
+
+val merkleTreeGenerationL0: #a: eqtype ->k: nat ->  l: list a {List.length l = pow2 k }->
+    Tot (r: list (merklePair #a 0) {List.length r = List.length l})
+
+let merkleTreeGenerationL0 #a k l = 
+    _merkleTreeGenerationL0 #a l
+
+val _merkleTreeGenerationLn: #a: eqtype -> level: nat-> l: list (merklePair #a level) {List.length l % 2 = 0}->
+    ML (r: list (merklePair #a (level+1)){List.length r = List.length l /2})
+    (*Tot(r: list (merklePair #a (level+1)) {List.length l = pow2 (k-1)})*)
+
+let rec _merkleTreeGenerationLn #a level l = 
+    assert (List.length l % 2 = 0);
+    match l with 
+    | hd::hd1::tl -> let (|hd_hash,hd_body|) = hd in 
+                     let (|hd1_hash, hd1_body|) = hd1 in 
+                     let node = MNode #a #level #hd_hash #hd1_hash hd_body hd1_body in
+                     let hash = concat hd_hash hd1_hash in 
+                     let element = (|hash, node|) in 
+                     assert(List.length tl = List.length l - 2); 
+                     List.append [element] (_merkleTreeGenerationLn #a level tl)
+    | [] -> []
+
+
+val merkleTreeGenerationLn: #a: eqtype -> level: nat -> k: nat -> l: list(merklePair #a level) {List.length l = pow2 k /\ k>0} ->
+    ML (r:list (merklePair #a (level +1)) {List.length r = pow2 (k-1)})
+
+let merkleTreeGenerationLn #a level k l = 
+    _merkleTreeGenerationLn #a level l 
+
+val _merkleListGeneration: #a: eqtype -> level: nat -> k: nat -> l: list(merklePair #a level){List.length l = pow2 k /\ k > 0} -> ML (hash_t)
+let rec _merkleListGeneration #a level k l = 
+    let l_new = merkleTreeGenerationLn #a level k l in  
+        assert (List.length l_new = pow2 (k-1)); 
+    if (List.length l_new = 1) then
+            (    
+                assert ((k-1) = 0);
+                let elem = hd l_new in 
+                let (|hash, b|) = elem 
+                in hash
+            )
+    else if (List.length l_new > 1) then 
+        (
+            assert ((k-1) > 0);
+            _merkleListGeneration #a (level+1) (k-1) l_new
+        )
+    else 
+        Seq.createEmpty
+
+val merkleListGeneration: #a: eqtype -> k: nat ->  l: list a{List.length l = pow2 k} -> ML (hash_t)
+let merkleListGeneration #a k l = 
+    let treeLeafs = merkleTreeGenerationL0 #a k l in 
+    if (List.length treeLeafs = 1) then 
+            (
+                let elem = hd treeLeafs in 
+                let (|hash, body|) = elem in 
+                hash
+            )
+    else 
+        (
+            assert (k>0);
+             _merkleListGeneration #a 0 k treeLeafs
+        )
